backend/Linear.v
@@ -291,7 +291,8 @@ Inductive step: state -> trace -> state -> Prop :=
       step (Callstate s (External ef) rs1 m)
          t (Returnstate s rs2 m')
   | exec_return:
-      forall s f sp rs0 c rs m,
+      forall s f sp rs0 c rs m
+      (Hnot_empty:not_empty s),
       step (Returnstate (Stackframe f sp rs0 c :: s) rs m)
         E0 (State s f sp c rs m).
 
@@ -306,26 +307,66 @@ Inductive initial_state (p: program): state -> Prop :=
       funsig f = signature_main ->
       initial_state p (Callstate nil f (Locmap.init Vundef) m0).
 
-(* This lets the stack frame for a spawned thread be an arbitrary internal function, but in fact
-   it should be fixed or possibly passed as an argument to entry_point. *)
+(*
+Definition pre_main_sig: signature:=
+  {| sig_args := nil;
+     sig_res := None ;
+     sig_cc := cc_default |}.
+*)
+Definition pre_main (stck_sz:Z): function:=
+  {| fn_sig := pre_main_sig;
+     fn_stacksize := stck_sz;
+     fn_code := nil |}.
+(* loc_arguments takes a signature, 
+   It generally only needs the types of arguemtns targs.
+   For RISC-V, it also takes calling conventions.
+ *)
+Definition pre_main_locset targs args: locset:=
+  let sg:= {| sig_args := targs;
+              sig_res := None;
+              sig_cc := cc_default |} in
+  build_ls_from_arguments sg args.
+Definition arg_size (args : list typ):= Z.of_nat (Datatypes.length args).
+Definition pre_main_stack targs args: stackframe:=
+  Stackframe
+    (pre_main (arg_size targs))
+    Vundef                     (* no stack pointere for pre_main *)
+    (pre_main_locset targs args) (* empty environment in pre_main *)
+    nil.                       (* No continuation in pre_main *)
+
+Definition pre_main_staklist sig args:=
+  (pre_main_stack sig args)::nil.
+Definition has_pre_main (cs:list stackframe):= (0 < length cs)%nat.
+Lemma has_pre_main_cons:
+  forall hd tl, has_pre_main (hd::tl).
+Proof. intros. unfold has_pre_main. simpl; omega. Qed.
+(* Move to RTL.v*)
+Lemma nil_has_pre_main:
+      has_pre_main nil -> False.
+Proof. unfold has_pre_main; simpl; omega. Qed.
+
+
+
 Inductive entry_point (p: program): mem -> state -> val -> list val -> Prop :=
-  | entry_point_intro: forall fb f m0 m1 stk args,
+  | entry_point_intro: forall fb f m0 m1 stk args targs,
       let ge := Genv.globalenv p in
       Mem.mem_wd m0 ->
       globals_not_fresh ge m0 ->
-      Mem.arg_well_formed args m0 ->
       Genv.find_funct_ptr ge fb = Some (Internal f) ->
       Val.has_type_list args (sig_args (funsig (Internal f))) ->
-(*      size_arguments (funsig f) <= Z.max (max_over_instrs outgoing_space) 
-        (max_over_slots_of_funct outgoing_slot) ->*)
+      (* Allocate a stackframe, to pass arguments in the stack*)
       Mem.alloc m0 0 0 = (m1, stk) ->
+      targs = sig_args (fn_sig f) ->
+      Val.has_type_list args targs -> 
       let ls := LTL.build_ls_from_arguments (funsig (Internal f)) args in
-      entry_point p m0 (Callstate nil (Internal f) ls m1) (Vptr fb Ptrofs.zero) args.
+      entry_point p m0 (Callstate (pre_main_staklist targs args)
+                                  (Internal f) ls m1)
+                  (Vptr fb Ptrofs.zero) args.
 
 Inductive final_state: state -> int -> Prop :=
-  | final_state_intro: forall rs m retcode,
+  | final_state_intro: forall rs m retcode pre_main,
       Locmap.getpair (map_rpair R (loc_result signature_main)) rs = Vint retcode ->
-      final_state (Returnstate nil rs m) retcode.
+      final_state (Returnstate (pre_main::nil) rs m) retcode.
 
 Definition semantics (p: program) :=
   let ge:= (Genv.globalenv p) in
